1. Caught RamifyCoq up to the latest VST (8a301dcc on Feb 21). Two issues remain here:   (i) We have been forced to downgrade back to Coq 8.8.1. This means that we currently need to change the Makefile each time we pull VST.   (ii) There are warnings that I know how to remove, but which are tedious to the extreme. Will get rid of them slowly. 2. Is_from is now proved to not get stuck. test_int_or_ptr does appear to be stuck.

CertiGC/verif_Is_from.v
@@ -34,12 +34,20 @@ Definition Is_from_sig : signature :=
 Lemma intmod_eq_ptrofsmod: Int.modulus = Ptrofs.modulus.
 Proof. now unfold Archi.ptr64; apply Ptrofs.modulus_eq32. Qed.
 
-Lemma lt_ptr_mod: forall n1 n2,
-    n1 <= n2 <= Ptrofs.max_unsigned -> n1 <= n2 < Ptrofs.modulus.
+Lemma lt_ptr_mod: forall n1 n2, n1 <= n2 <= Ptrofs.max_unsigned -> n1 <= n2 < Ptrofs.modulus.
 Proof.
   intros.
   replace Ptrofs.max_unsigned with (Z.pred Ptrofs.modulus) in * by rep_omega.
   now rewrite <- Z.lt_le_pred in *.
+Qed.
+
+Lemma mem_ext_valid_block: forall m1 m2 b i n,
+    Mem.extends m1 m2 -> valid_block m1 b i n -> valid_block m2 b i n.
+Proof.
+  intros. destruct H0 as [? [? ?]].
+  do 2 (split; trivial).
+  intros. specialize (H2 i0 H3).
+  eapply Mem.valid_pointer_extends; eauto.
 Qed.
 
 Lemma Is_from_extcall: extcall_properties Is_from_sem Is_from_sig.
@@ -49,116 +57,96 @@ Proof.
     do 4 (destruct vargs; try destruct v; try contradiction).
     destruct H as [_ [_ [_ [_ [_ [_ [_ ?]]]]]]].
     destruct H as [[_ [_ ?]] | [_ ?]]; subst; apply I.
-  - intros. apply H0.
-  - intros. destruct H as [? _]. subst m1. apply H0.
-  - intros. destruct H as [? _]. subst m1. apply H1.
-  - intros. destruct H as [? _]. subst m1.
-    apply Mem.unchanged_on_refl.
+  - intros; apply H0.
+  - intros. destruct H as [? _]. subst m1. trivial. 
+  - intros. destruct H as [? _]. subst m1. trivial. 
+  - intros. destruct H as [? _]. subst m1; apply Mem.unchanged_on_refl.
   - intros. exists vres, m1'.
-    destruct H as [? [? ?]]. subst m2 t.
-    split. 2: { split. apply Val.lessdef_refl. split. trivial. apply Mem.unchanged_on_refl. }
-    split. trivial. split. trivial.
+    destruct H as [? [? ?]]; subst m2 t.
+    split.      
+    2: split3; [apply Val.lessdef_refl | trivial | apply Mem.unchanged_on_refl].
+    split3; trivial.
     do 4 (destruct vargs; try destruct v; try contradiction).    
-    inversion H1. inversion H4. inversion H6. inversion H11.
-    inversion H13. inversion H18. inversion H20. subst. clear H4 H11 H18 H20 H13 H6 H1.
+    inversion H1; inversion H4; inversion H6; inversion H11;
+      inversion H13; inversion H18; inversion H20; subst.
+    clear H4 H11 H18 H20 H13 H6 H1.
     destruct H3 as [n [? [? [? [? ?]]]]].
-    exists n. repeat (split; [assumption|]). clear H H1 H2 H3. 
-    destruct H4 as [? [? ?]].
-    split. {
-      clear -H H0.
-      destruct H as [? [? ?]]. do 2 (split; trivial).
-      intros i0 Hx. specialize (H2 i0 Hx).
-      eapply Mem.valid_pointer_extends; eauto. }
-    split. eapply Mem.valid_pointer_extends; eauto.
-    tauto.
+    exists n. do 4 (split; trivial).
+    clear -H0 H4. destruct H4 as [? [? ?]].
+    split3; [apply (mem_ext_valid_block _ _ _ _ _ H0 H) | eapply Mem.valid_pointer_extends; eauto | tauto].
   - intros. exists f, vres, m1'. destruct H0 as [? [? ?]]. 
     split.
     2: {
       split.
-      - do 4 (destruct vargs; try destruct v; try contradiction). inversion H2. inversion H7. inversion H9.
-      inversion H17. inversion H19.
-      inversion H27. inversion H29.
-      destruct H4 as [n [? [? [? [? [? [? ?]]]]]]]. 
-      destruct vres; auto.  
-      now destruct H41.
+      - clear -H4.
+        do 4 (destruct vargs; try destruct v; try contradiction).
+        destruct H4 as [_ [_ [_ [_ [_ [_ [_ H]]]]]]].
+        destruct vres; auto. now destruct H. 
       - repeat (split; [now subst|]).
         apply mem_lemmas.inject_separated_same_meminj.
     }
     split3; trivial.
     do 4 (destruct vargs; try destruct v; try contradiction).
     inversion H2; inversion H7; inversion H9;
-      inversion H17; inversion H19; inversion H27;
-        inversion H29; subst.
+      inversion H17; inversion H19; inversion H27; inversion H29; subst.
     clear H2 H7 H9 H17 H19 H27 H29.
     destruct H4 as [n [? [? [? [? [? [? ?]]]]]]].
-    subst. exists n. rewrite H22 in H12; inversion H12. subst.
-    clear H12.
-    assert (Hf: 0 <= Ptrofs.unsigned i + n < Ptrofs.modulus) by  
-        (unfold Ptrofs.unsigned, Ptrofs.intval; destruct i;
-         split; [omega | auto]).
+    exists n. rewrite H3 in  H12; rewrite H22 in H12; inversion H12.
+    subst; clear H12.
+    assert (Hf: 0 <= Ptrofs.unsigned i + n < Ptrofs.modulus) by
+        (rewrite H4; apply Ptrofs.unsigned_range).
     assert (Ha: Ptrofs.unsigned (Ptrofs.add i (Ptrofs.repr delta)) + n < Int.modulus). {
       rewrite intmod_eq_ptrofsmod.
       destruct H1 as [_ _ _ _ rep _].
-      generalize (rep b0 b3 delta
-                      (Ptrofs.add i (Ptrofs.repr n)) H22).
-      intros [Hx Hy].
+      destruct (rep b0 b3 delta
+                      (Ptrofs.add i (Ptrofs.repr n)) H22) as [Hx Hy]. 
       { right. apply Mem.perm_cur_max, Mem.valid_pointer_nonempty_perm.
         destruct H5 as [_ [_ H5]].
-        assert (Hm: 0 <= n - 1 < n) by omega.
-        rewrite <- (H5 _ Hm).
-        f_equal.
-        unfold Ptrofs.add; repeat rewrite Ptrofs.unsigned_repr_eq.
-        rewrite Z.add_mod_idemp_r, Z.mod_small by easy. omega. }
-      clear -Hy Hf H0 Hx.
+        assert (Hm: 0 <= n - 1 < n) by omega; rewrite <- (H5 _ Hm).
+        f_equal; unfold Ptrofs.add; repeat rewrite Ptrofs.unsigned_repr_eq.
+        rewrite Z.add_mod_idemp_r, Z.mod_small by easy. omega.
+      }
+      clear -Hx Hy Hf H0.
       apply lt_ptr_mod in Hy.
-      destruct Hy as [Hy' Hy].
-      unfold Ptrofs.add in *.
+      unfold Ptrofs.add in *. 
       repeat rewrite Ptrofs.unsigned_repr_eq in *.
-      rewrite Z.add_mod_idemp_r, Z.mod_small in Hy, Hy' by easy.
-      rewrite Z.add_mod_idemp_r by easy.
-      rewrite Z.mod_small; [omega|].
+      rewrite Z.add_mod_idemp_r, Z.mod_small in * by easy.
+      rewrite Z.mod_small; [omega|]. 
       destruct i. unfold Ptrofs.unsigned in *; simpl in *. omega.
     }
     split3; [| |split3; [| |split3]]; trivial.
-    + unfold Ptrofs.add. rewrite <- H4.
+    + destruct H1 as [_ _ _ _ rep _].
+      destruct (rep _ _ delta
+                   (Ptrofs.add i (Ptrofs.repr n)) H22) as [Hd' Hd]. {
+        right. apply Mem.perm_cur_max, Mem.valid_pointer_nonempty_perm.
+        destruct H5 as [_ [_ H5]]. assert (0 <= n - 1 < n) by omega.
+        rewrite <- (H5 _ H1). f_equal.
+        unfold Ptrofs.add; repeat rewrite Ptrofs.unsigned_repr_eq.
+        rewrite Z.add_mod_idemp_r, Z.mod_small by easy. omega.
+      }
+      unfold Ptrofs.add. rewrite <- H4.
       destruct (Ptrofs.unsigned_range i) as [? _].
       repeat rewrite Ptrofs.unsigned_repr_eq.
       repeat rewrite Z.add_mod_idemp_r by easy.
       rewrite intmod_eq_ptrofsmod in Ha.
-      destruct H1 as [_ _ _ _ rep _].
-      destruct (rep _ _ delta
-                   (Ptrofs.add i (Ptrofs.repr n)) H22) as [Hd' Hd]. {
-        right. apply Mem.perm_cur_max, Mem.valid_pointer_nonempty_perm.
-        destruct H5 as [_ [_ H5]].
-        assert (0 <= n - 1 < n) by omega.
-        rewrite <- (H5 _ H1). f_equal.
-        unfold Ptrofs.add. repeat rewrite Ptrofs.unsigned_repr_eq.
-        rewrite Z.add_mod_idemp_r, Z.mod_small by easy.
-        omega.
-      }
       unfold Ptrofs.add in Hd.
       repeat rewrite Ptrofs.unsigned_repr_eq in Hd.
       rewrite Z.add_mod_idemp_r, Z.mod_small in Hd by easy.
       apply lt_ptr_mod in Hd.
       repeat rewrite Z.mod_small; [omega | trivial | omega].
     + split3; [easy | omega|]. intros.
-      destruct H5 as [_ [_ H5]]. assert (Hs := H5).
-      specialize (H5 i2 H3).
-      rewrite <- (Mem.valid_pointer_inject _ _ _ _ _ _ _ H22 H1 H5).
-      f_equal. unfold Ptrofs.add.
-      repeat rewrite Ptrofs.unsigned_repr_eq.
+      destruct H5 as [_ [_ H5]].
+      rewrite <- (Mem.valid_pointer_inject _ _ _ _ _ _ _ H22 H1 (H5 i2 H3)).
+      f_equal. unfold Ptrofs.add; repeat rewrite Ptrofs.unsigned_repr_eq.
       destruct H1 as [_ _ _ _ rep _].
       destruct (rep _ _ delta i H22) as [_ Hd]. {
         left. apply Mem.perm_cur_max, Mem.valid_pointer_nonempty_perm.
-        assert (0 <= 0 < n) by omega.
-        specialize (Hs 0 H1). rewrite <- Hs. f_equal. omega.
+        assert (0 <= 0 < n) by omega; rewrite <- (H5 0 H1); f_equal; omega.
       } 
       apply lt_ptr_mod in Hd.
-      rewrite Z.add_mod_idemp_r by easy.
-      rewrite Z.mod_small by easy. omega.
+      rewrite Z.add_mod_idemp_r, Z.mod_small by easy. omega.
     + rewrite <- (Mem.valid_pointer_inject _ _ _ _ _ _ _ H32 H1 H6).
-      f_equal. unfold Ptrofs.add.
-      repeat rewrite Ptrofs.unsigned_repr_eq.
+      f_equal. unfold Ptrofs.add. repeat rewrite Ptrofs.unsigned_repr_eq.
       destruct H1 as [_ _ _ _ rep _].
       destruct (rep _ _ delta1 i1 H32) as [_ Hd]. {
         left; now apply Mem.perm_cur_max,
@@ -167,27 +155,25 @@ Proof.
       apply lt_ptr_mod in Hd.
       rewrite Z.add_mod_idemp_r, Z.mod_small by easy. omega.
     + destruct H7.
-      * destruct H3 as [? [? ?]].
+      * destruct H3 as [? [? ?]]; subst b1 vres.
         destruct H1 as [_ _ _ _ rep _].
         destruct (rep b0 b3 delta i H22) as [_ Hp]. {
           left; apply Mem.perm_cur_max, Mem.valid_pointer_nonempty_perm.
-          destruct H5 as [_ [_ H1]]; assert (H5: 0 <= 0 < n) by omega.
-          specialize (H1 0 H5).
-          now replace (Ptrofs.unsigned i + 0) with (Ptrofs.unsigned i) in H1 by omega.
+          destruct H5 as [_ [_ H5]]; assert (0 <= 0 < n) by omega.
+          specialize (H5 0 H1).
+          now replace (Ptrofs.unsigned i + 0) with (Ptrofs.unsigned i) in H5 by omega.
         }
         destruct (rep b0 b3 delta i1 H22) as [_ Hq]. {
           left; apply Mem.perm_cur_max, Mem.valid_pointer_nonempty_perm;
             destruct H5 as [_ [_ ?]]; assert (0 <= 0 < n) by omega.
-          specialize (H1 0 H5); now rewrite H3.
+          specialize (H1 0 H3); now rewrite H6.
         }
         destruct (rep b0 b3 delta i0 H22) as [_ Hr]. {
-          destruct H5 as [_ [_ H5]].
-          rewrite <- H4.
+          destruct H5 as [_ [_ H5]]. rewrite <- H4.
           assert (Hm: 0 <= n - 1 < n) by omega.
           right. apply Mem.perm_cur_max, Mem.valid_pointer_nonempty_perm.
           rewrite <- (H5 _ Hm); f_equal; omega.
         }
-        subst b0.
         rewrite H22 in H32; inversion H32.
         left. split3; trivial.
         subst delta1. clear -H7 Hp Hq Hr.
@@ -196,72 +182,58 @@ Proof.
         repeat rewrite Z.add_mod_idemp_r, Z.mod_small by easy.
         omega.
       * destruct H3. right. split; trivial.
-        rename m2 into m. rename m1' into m'.
-        destruct H1 as [[perm _ _] _ _ lap rep inv].
+        rename m2 into m; rename m1' into m'.
+        destruct H1 as [_ _ _ lap rep _].
         destruct H3.
-        -- destruct (EqDec_block b3 b7); [subst b3 | now left].
-           right; split; trivial.
+        -- destruct (EqDec_block b3 b7); [|now left].
+           subst b3. right. split; trivial.
            unfold Ptrofs.add; repeat rewrite Ptrofs.unsigned_repr_eq.
            repeat rewrite Z.add_mod_idemp_r by easy.
-           assert (Hs := H5).
            destruct H5 as [_ [_ H5]].
-           assert (bound: 0 <= 0 < n) by omega.
-           specialize (H5 _ bound).
-           clear bound.
+           assert (0 <= 0 < n) by omega.
+           pose proof (H5 _ H3).
            apply Mem.valid_pointer_nonempty_perm, Mem.perm_cur_max in H6.
-           apply Mem.valid_pointer_nonempty_perm, Mem.perm_cur_max in H5.
-           replace (Ptrofs.unsigned i + 0) with (Ptrofs.unsigned i) in H5 by omega.
-           (* specialize (lap b0 b7 delta b1 b7 delta1 (Ptrofs.unsigned i) (Ptrofs.unsigned i1) H3 H22 H32 H5 H6). (**) *)
-           specialize (lap _ _ _ _ _ _ _ _ H1 H22 H32 H5 H6). (**)
-           destruct (rep _ _ delta1 i1 H32) as [_ Hp].
-           1: left; easy.
-           destruct (rep _ _ delta i H22) as [_ Hq].
-           1: left; easy.
+           apply Mem.valid_pointer_nonempty_perm, Mem.perm_cur_max in H8.
+           replace (Ptrofs.unsigned i + 0) with (Ptrofs.unsigned i) in H8 by omega.
+           destruct (rep _ _ delta1 i1 H32) as [_ Hp]; [left; easy|].
+           destruct (rep _ _ delta i H22) as [_ Hq]; [left; easy|].
            destruct (rep _ _ delta i0 H22) as [_ Hr]. {
-             destruct Hs as [_ [_ Hs]]. 
              rewrite <- H4.
              assert (Hm: 0 <= n - 1 < n) by omega.
-             specialize (Hs _ Hm).
-             replace (Ptrofs.unsigned i + (n - 1)) with (Ptrofs.unsigned i + n - 1) in Hs by omega.
-             apply Mem.valid_pointer_nonempty_perm, Mem.perm_cur_max in Hs. now right.
+             specialize (H5 _ Hm).
+             replace (Ptrofs.unsigned i + (n - 1)) with (Ptrofs.unsigned i + n - 1) in H5 by omega.
+             apply Mem.valid_pointer_nonempty_perm, Mem.perm_cur_max in H5. now right.
            }
            replace Ptrofs.max_unsigned with (Z.pred Ptrofs.modulus) in * by rep_omega.
            rewrite <- Z.lt_le_pred in *.
            repeat rewrite Z.mod_small by easy.
-           destruct lap as [? | lap]; [contradiction|].
+           destruct (lap _ _ _ _ _ _ _ _ H1 H22 H32 H8 H6); [contradiction|].
            clear rep Hp Hq Hr.
            replace (Ptrofs.unsigned i) with ((Ptrofs.unsigned i - delta) + delta) in H5 by omega.
-           destruct Hs as [_ [_ Hs]].
-           specialize (perm b0 b7 delta (Ptrofs.unsigned i - delta) Max Nonempty H22).
-           specialize (inv _ (Ptrofs.unsigned i - delta) _ _ Max Nonempty H22).
-           (* Hrm... kinda worked myself into a corner.
-            * Feels circular and weird. 
-            * Consider perm --> inv.
-            * Plus, specializing Hs is hard 
-            *   cuz I would want "-delta" for i0, 
-            *   and good luck proving the bound for that.
-            *)
-           (* stuck.
-            * too many seemingly unrelated variables
-            * and no disjunction above the bar.
-            *)
-           admit.
-        -- destruct H3. subst b0.
-           right. rewrite H22 in H32; inversion H32.
+           assert ((Ptrofs.unsigned i1 + delta1 < Ptrofs.unsigned i + delta) \/
+                   (Ptrofs.unsigned i1 + delta1 >= Ptrofs.unsigned i0 + delta) \/
+                   ((Ptrofs.unsigned i1 + delta1 >= Ptrofs.unsigned i + delta) /\
+                    Ptrofs.unsigned i1 + delta1 < Ptrofs.unsigned i0 + delta)) by omega.
+           destruct H10; [auto | destruct H10; [auto|]]. exfalso.
+           destruct H10. rewrite <- H4 in H11.
+           assert (0 <= Ptrofs.unsigned i1 + delta1 - Ptrofs.unsigned i - delta < n) by omega.
+           specialize (H5 (Ptrofs.unsigned i1 + delta1 - Ptrofs.unsigned i - delta) H12).
+           apply Mem.valid_pointer_nonempty_perm, Mem.perm_cur_max in H5.
+           destruct (lap b0 b7 delta b1 b7 delta1 _ (Ptrofs.unsigned i1) H1 H22 H32 H5 H6); [auto | apply H13; omega].
+        -- destruct H1. subst b0 vres.
+           right. rewrite H22 in H32; inversion H32. clear H32.
            split; trivial.
            unfold Ptrofs.add; repeat rewrite Ptrofs.unsigned_repr_eq.
            repeat rewrite Z.add_mod_idemp_r by easy.
-           destruct H1 as [_ _ _ _ rep _].
            subst delta1.           
            destruct (rep b1 b3 delta i H22) as [_ Hp]. {
              left; apply Mem.perm_cur_max, Mem.valid_pointer_nonempty_perm.
-             destruct H5 as [_ [_ H1]]; assert (H5: 0 <= 0 < n) by omega.
-             specialize (H1 0 H5).
-             now replace (Ptrofs.unsigned i + 0) with (Ptrofs.unsigned i) in H1 by omega.
+             destruct H5 as [_ [_ H5]]; assert (H1: 0 <= 0 < n) by omega.
+             specialize (H5 0 H1).
+             now replace (Ptrofs.unsigned i + 0) with (Ptrofs.unsigned i) in H5 by omega.
            }
-           destruct (rep b1 b3 delta i1 H22) as [_ Hq]. {
-             now left; apply Mem.perm_cur_max, Mem.valid_pointer_nonempty_perm.
-           }
+           destruct (rep b1 b3 delta i1 H22) as [_ Hq].
+           1:  now left; apply Mem.perm_cur_max, Mem.valid_pointer_nonempty_perm.
            destruct (rep b1 b3 delta i0 H22) as [_ Hr]. {
              destruct H5 as [_ [_ H5]].
              rewrite <- H4.
@@ -269,35 +241,77 @@ Proof.
              right. apply Mem.perm_cur_max, Mem.valid_pointer_nonempty_perm.
              rewrite <- (H5 _ Hm); f_equal; omega.
            }
-           clear - H8 Hp Hq Hr.
+           clear - H3 Hp Hq Hr.
            apply lt_ptr_mod in Hp; apply lt_ptr_mod in Hq; apply lt_ptr_mod in Hr. 
            repeat rewrite Z.mod_small by easy.
-           destruct H8; [left | right]; omega.
-(** External calls must commute with memory injections,
-  in the following sense.
-  ec_mem_inject:
-    forall ge1 ge2 vargs m1 t vres m2 f m1' vargs',
-    symbols_inject f ge1 ge2 ->
-    sem ge1 vargs m1 t vres m2 ->
-    Mem.inject f m1 m1' ->
-    Val.inject_list f vargs vargs' ->
-    exists f', exists vres', exists m2',
-       sem ge2 vargs' m1' t vres' m2'
-    /\ Val.inject f' vres vres'
-    /\ Mem.inject f' m2 m2'
-    /\ Mem.unchanged_on (loc_unmapped f) m1 m2
-    /\ Mem.unchanged_on (loc_out_of_reach f m1) m1' m2'
-    /\ inject_incr f f'
-    /\ inject_separated f f' m1 m1';
-       *)
+           destruct H3; [left | right]; omega.
   - intros. destruct H as [_ [? _]]. subst t. simpl. omega.
   - intros. generalize H. destruct H as [_ [? _]]. subst t1. inversion H0. subst t2. clear H0. intro H.
-      exists vres1, m1. apply H.
+    exists vres1, m1. apply H.
   - intros. destruct H as [? [? ?]]. destruct H0 as [? [? ?]].
-      subst m1 m2 t1 t2. split. constructor. intros _.
-      split; trivial.
-      do 4 (destruct vargs; try destruct v; try contradiction).
-      destruct H2 as [_ [_ [_ [_ [_ [_ [_ ?]]]]]]].
-      destruct H4 as [_ [_ [_ [_ [_ [_ [_ ?]]]]]]].
-      intuition; congruence.
+    subst m1 m2 t1 t2.
+    split; [constructor|].
+    intros _. split; trivial.
+    do 4 (destruct vargs; try destruct v; try contradiction).
+    destruct H2 as [_ [_ [_ [_ [_ [_ [_ ?]]]]]]].
+    destruct H4 as [_ [_ [_ [_ [_ [_ [_ ?]]]]]]].
+    intuition; congruence.
+Qed.
+
+Definition test_iop_sem : extcall_sem :=
+  fun _ args m1 trc ret m2 =>
+    m1 = m2 /\ trc = nil /\ 
+    match args with
+    | (Vint i) :: [] =>
+      ret = Vint (Int.modu i (Int.repr 2))
+    | (Vptr b ofs) :: [] =>
+      ret = Vint (Ptrofs.to_int (Ptrofs.modu ofs (Ptrofs.repr 2)))
+    | _ => False
+    end.
+
+Definition test_iop_sig : signature :=
+  mksignature (AST.Tint :: nil) (Some AST.Tint) cc_default.
+
+Lemma test_iop__extcall: extcall_properties test_iop_sem test_iop_sig.
+Proof.
+  constructor.
+  - intros. destruct H as [_ [_ ?]].
+    do 2 (destruct vargs; try destruct v; try contradiction); subst; apply I.
+  - intros. apply H0.
+  - intros. destruct H as [? _]. subst m1. trivial. 
+  - intros. destruct H as [? _]. subst m1. trivial.
+  - intros. destruct H as [? _]. subst m1. apply Mem.unchanged_on_refl.
+  - intros. exists vres, m1'.
+    destruct H as [? [? ?]]. subst m2 t.
+    split.
+    2: split3; [apply Val.lessdef_refl | trivial | apply Mem.unchanged_on_refl]. 
+    split3; trivial.
+    do 2 (destruct vargs; try destruct v; try contradiction);    
+      inversion H1; inversion H4; inversion H6; auto.
+  - intros. (* is the choice of f forced?? *)
+    exists f, vres, m1'. destruct H0 as [? [? ?]]; subst.
+    split.
+    2: {
+      split.
+      - do 2 (destruct vargs; try destruct v; try contradiction); subst; constructor.
+      - split; [trivial|].
+        split; [apply Mem.unchanged_on_refl|].
+        split; [apply Mem.unchanged_on_refl|].
+        split; [apply inject_incr_refl|].
+        apply mem_lemmas.inject_separated_same_meminj.
+    } clear f H H1 H2.
+    split3; trivial.
+    do 2  (destruct vargs; try destruct v; try contradiction).
+    + inversion H2; inversion H5; inversion H7; trivial.
+    + inversion H2; inversion H5; inversion H7; subst.
+      (* dead *)
+      admit.
+  - intros. destruct H as [_ [? _]]. subst t. simpl; omega.
+  - intros. generalize H. destruct H as [_ [? _]].
+    subst t1; inversion H0; subst t2.
+    intro H; exists vres1, m1; apply H.
+  - intros. destruct H as [? [? ?]]. destruct H0 as [? [? ?]].
+    subst m1 m2 t1 t2.
+    split; [constructor|]. intros _. split; trivial.
+    do 2 (destruct vargs; try destruct v; try contradiction); congruence.
 Admitted.
